proofs/FEC/DecoderTimeouts.v
@@ -90,7 +90,6 @@ Definition bounded_reorder_list (rec: list fpacket):=
   (nat_abs_diff (u_seqNum rec p1) (u_seqNum rec p2) <= (k + h) + 2 * d)%N.
 
 (*TODO: move*)
-Print u_seqNum.
 Lemma u_seqNum_cat_in: forall {A: eqType} (l1 l2: seq A) (x: A),
   x \in l1 ->
   u_seqNum (l1 ++ l2) x = u_seqNum l1 x.
@@ -196,35 +195,9 @@ Proof.
 Qed. 
 
 (*TODO move these*)
-Lemma create_black_time: forall p time,
-  black_time (create_block_with_packet_black p time).1 = time.
-Proof.
-  move=> p time /=.
-  by case: (Z.eq_dec (fd_k p) 1).
-Qed.
 
-Lemma create_black_id: forall p time,
-  blk_id (create_block_with_packet_black p time).1 = fd_blockId p.
-Proof.
-  move=> p time/=.
-  by case: (Z.eq_dec (fd_k p) 1).
-Qed.
 
-Lemma add_black_time: forall p b,
-  black_time (add_packet_to_block_black p b).1 = black_time b.
-Proof.
-  move=> p b. rewrite /add_packet_to_block_black.
-  case: (black_complete b)=>//.
-  by case: (recoverable (add_fec_packet_to_block p b)).
-Qed.
 
-Lemma add_black_id: forall p b,
-  blk_id (add_packet_to_block_black p b).1 = blk_id b.
-Proof.
-  move=>p b. rewrite /add_packet_to_block_black.
-  case:(black_complete b)=>//.
-  by case: (recoverable (add_fec_packet_to_block p b)).
-Qed.
 
 (*We need several sets of invariants to prove what we want
   (that under the reordering assumptions, the decoder is equivalent
@@ -263,6 +236,71 @@ Qed.
   (forall b, b \in blocks -> exists b', b' \in (get_blocks prev) /\
     subblock b b').
 
+(*A key lemma that we need for our invariant: a packet with the
+  same blockId as the current block could not have appeared too
+  far in the past*)
+Lemma same_block_close: forall prev (p p1: fpacket) l1 l2,
+  reorder_dup_cond (prev ++ [:: p]) ->
+  prev = l1 ++ [:: p1] ++ l2 ->
+  p1 \notin l1 ->
+  fd_blockId p1 = fd_blockId p ->
+  ~(Z.of_nat (size (undup_fst (l1 ++ [:: p1] ++ l2 ++ [:: p]))) -
+    Z.of_nat (size (undup_fst (l1 ++ [:: p1]))) > threshold).
+Proof.
+  move=> prev p p1 l1 l2.
+  rewrite /reorder_dup_cond/bounded_reorder_list/duplicates_bounded =>
+  [[Hreord [Hdups Hthresh]]] Hprev Hnotin1 Hids.
+  have Hcon: ((size (undup_fst (l1 ++ [:: p1] ++ l2 ++ [:: p])) - 
+    size (undup_fst (l1 ++ [:: p1])))%N <= 
+    (k + h + 2 * d) + dup)%N. {
+      eapply (@packets_reorder_dup_bound' _ (prev ++ [:: p]) fpacket_inhab
+        (fun (x: fpacket) =>  (x \in prev ++ [:: p]) 
+          && (fd_blockId x == fd_blockId p)) _ _) with(p2:=p)(l3:=nil) =>//.
+      - move=> pa pb /andP[Hinpa /eqP Hidpa] /andP[Hinpb /eqP Hidpb].
+        apply Hreord=>//. by rewrite Hidpa Hidpb.
+      - by rewrite cats0 Hprev -catA.
+      - by rewrite Hids Hprev !mem_cat in_cons !eq_refl !orbT.
+      - by rewrite mem_cat in_cons !eq_refl !orbT.
+    }
+  (*Now we get an easy contradiction of inequalities*)
+  move=>Htimeout.
+  rewrite -Nat2Z.inj_sub in Htimeout.
+  - have /ltP: (size (undup_fst (l1 ++ [:: p1] ++ l2 ++ [:: p])) - 
+      size (undup_fst (l1 ++ [:: p1])) > k + h + 2 * d + dup)%coq_nat. {
+      apply Nat2Z.inj_gt. eapply Zgt_le_trans. apply Htimeout. lia.
+    }
+    by rewrite ltnNge Hcon.
+  - rewrite catA. apply /leP. apply size_undup_fst_le_app.
+Qed. 
+
+(*TODO: could move to BLocks maybe*)
+Lemma decoder_invar_allid: forall (blocks : seq block) prev,
+  wf_packet_stream prev ->
+  (forall b, b \in blocks -> exists b', b' \in (get_blocks prev) /\
+  subblock b b') ->
+  forall (b' : block) (p0 : fpacket),
+  b' \in blocks -> packet_in_block p0 b' -> fd_blockId p0 = blk_id b'.
+Proof.
+  move=> blocks prev Hwf Hsubblock b p' Hinb Hinp'.
+  move: Hsubblock=> /(_ b Hinb) [b' [Hinb' Hsubb]].
+  have Hinb2:= (subblock_in Hsubb Hinp').
+  rewrite (proj1 Hsubb).
+  by apply (get_blocks_ids Hwf).
+Qed.
+(*same*)
+Lemma decoder_invar_inprev: forall (blocks: seq block) prev,
+  wf_packet_stream prev ->
+  (forall b, b \in blocks -> exists b', b' \in (get_blocks prev) /\
+  subblock b b') ->
+  forall (b: block) (p: fpacket),
+    b \in blocks -> packet_in_block p b -> p \in prev.
+Proof.
+  move=> blocks prev Hwf Hsubblock b p' Hinb Hinpb'.
+  move: Hsubblock => /(_ b Hinb) [b1 [Hinb1 Hsub]].
+  apply (get_blocks_in_orig Hwf Hinb1).
+  apply (subblock_in Hsub Hinpb').
+Qed.
+
 (*We prove that this invariant is preserved. This is the key
   structural lemma to characterize the timeout behavior*)
   Lemma decoder_timeout_invar_preserved_one: forall blocks prev time p,
@@ -284,54 +322,9 @@ Proof.
   have Hwf': wf_packet_stream prev by
     apply (wf_packet_stream_tl Hwfcons). 
   (*All packets in blocks agree with ID values*)
-  have Hallid: forall (b' : block) (p0 : fpacket),
-    b' \in blocks -> packet_in_block p0 b' -> fd_blockId p0 = blk_id b'. {
-    move=> b p' Hinb Hinp'.
-    move: Hsubblock=> /(_ b Hinb) [b' [Hinb' Hsubb]].
-    have Hinb2:= (subblock_in Hsubb Hinp').
-    rewrite (proj1 Hsubb).
-    by apply (get_blocks_ids Hwf').
-  }
+  have Hallid:= (decoder_invar_allid Hwf' Hsubblock).
   (*All packets in a block are in prev*)
-  have Hinprev: forall (b: block) (p: fpacket),
-    b \in blocks -> packet_in_block p b -> p \in prev. {
-      move=> b p' Hinb Hinpb'.
-      move: Hsubblock => /(_ b Hinb) [b1 [Hinb1 Hsub]].
-      apply (get_blocks_in_orig Hwf' Hinb1).
-      apply (subblock_in Hsub Hinpb').
-  }
-  (*A key result that we use in several places and which underlies
-    the entire invariant: we cannot have a packet in the same block
-    as the current packet that arrived too much earlier*)
-  have Hclose: forall (p1 (*p2*): fpacket) l1 l2,
-    prev (*++ [:: p]*) = l1 ++ [:: p1] ++ l2 (*++ [:: p2]*) ->
-    p1 \notin l1 ->
-    fd_blockId p1 = fd_blockId p ->
-    ~(Z.of_nat (size (undup_fst (l1 ++ [:: p1] ++ l2 ++ [:: p]))) -
-    Z.of_nat (size (undup_fst (l1 ++ [:: p1]))) > threshold). {
-      move=> p1 l1 l2 Hprev Hnotin1 Hids.
-      have Hcon: ((size (undup_fst (l1 ++ [:: p1] ++ l2 ++ [:: p])) - 
-        size (undup_fst (l1 ++ [:: p1])))%N <= 
-        (k + h + 2 * d) + dup)%N. {
-          eapply (@packets_reorder_dup_bound' _ (prev ++ [:: p]) fpacket_inhab
-            (fun (x: fpacket) =>  (x \in prev ++ [:: p]) 
-              && (fd_blockId x == fd_blockId p)) _ _) with(p2:=p)(l3:=nil) =>//.
-          - move=> pa pb /andP[Hinpa /eqP Hidpa] /andP[Hinpb /eqP Hidpb].
-            apply Hreord=>//. by rewrite Hidpa Hidpb.
-          - by rewrite cats0 Hprev -catA.
-          - by rewrite Hids Hprev !mem_cat in_cons !eq_refl !orbT.
-          - by rewrite mem_cat in_cons !eq_refl !orbT.
-        }
-      (*Now we get an easy contradiction of inequalities*)
-      move=>Htimeout.
-      rewrite -Nat2Z.inj_sub in Htimeout.
-      - have /ltP: (size (undup_fst (l1 ++ [:: p1] ++ l2 ++ [:: p])) - 
-          size (undup_fst (l1 ++ [:: p1])) > k + h + 2 * d + dup)%coq_nat. {
-          apply Nat2Z.inj_gt. eapply Zgt_le_trans. apply Htimeout. lia.
-        }
-        by rewrite ltnNge Hcon.
-      - rewrite catA. apply /leP. apply size_undup_fst_le_app. 
-    }
+  have Hinprev:= (decoder_invar_inprev Hwf' Hsubblock). 
   (*We do the 1st invariant separately, since it's useful
     in the rest*)
   have Hupdtime: (upd_time time p blocks = Z.of_nat (size (undup_fst (prev ++ [:: p])))). {
@@ -350,7 +343,7 @@ Proof.
           by rewrite size_cat/= Nat2Z.inj_add/= Htime.
         move: Hprevnotin => /(_ p Hpinprev Hnotin) 
           [p' [l1 [l2 [Hidpp'[Hprev [Hnotinp' Htimeout]]]]]].
-        exfalso. apply (Hclose p' (*p*) l1 l2 (*nil*))=>//. 
+        exfalso. apply (@same_block_close prev p p' (*p*) l1 l2 (*nil*))=>//. 
         have->: l1 ++ [:: p'] ++ l2 ++ [:: p] = prev ++ [:: p] by
           rewrite !catA -(catA l1) Hprev.
         by rewrite !undup_fst_rcons Hpinprev (negbTE Hnotinp') 
@@ -398,7 +391,7 @@ Proof.
             [p' [l1 [l2 [Hidp' [Hprev [Hnotinp' Htimeb']]]]]].
           rewrite Z.leb_antisym => Hto. apply negbFE in Hto.
           move: Hto => /Z.ltb_spec0. rewrite Hprev -Htimeb' => Hcon.
-          exfalso. apply (Hclose p' (*p*) l1 l2 (*nil*))=>//.
+          exfalso. apply (@same_block_close prev p p' (*p*) l1 l2 (*nil*))=>//.
           by rewrite Hpid Hidp'.
           rewrite undup_fst_rcons (negbTE Hnotinp') size_cat/=addn1.
           rewrite -!catA in Hcon. simpl in *; lia.
@@ -407,7 +400,7 @@ Proof.
           move => Hnotex.
           move: Hprevnotin => /(_ p Hinp Hnotex) 
             [p' [l1 [l2 [Hideq [Hprev [Hnotinp' Htimeout]]]]]].
-          exfalso. apply (Hclose p' l1 l2)=>//.
+          exfalso. apply (@same_block_close prev p p' l1 l2)=>//.
           have->:(l1 ++ [:: p'] ++ l2 ++ [:: p]) = prev ++ [:: p]
             by rewrite !catA -(catA l1) Hprev.
           by rewrite !undup_fst_rcons (negbTE Hnotinp') Hinp size_cat/= 
@@ -518,7 +511,7 @@ Proof.
     by rewrite -(perm_mem Hperm).
 Qed.
 
-Opaque decoder_one_step.
+(*Opaque decoder_one_step.*)
 
 (*Therefore, the invariant holds of [decoder_all_steps]*)
 Lemma decoder_timeout_invar_all: forall packets,
@@ -547,7 +540,6 @@ Qed.
   without timeouts (in terms of output). 
   The key idea is that all blocks that contain packets
   that might arrive later are kept*)
-Print decoder_multiple_steps_gen.
 
 (*let' see if this condition works first*)
 
@@ -577,7 +569,13 @@ Definition to_nto_invar (blks1 blks2 : list block)
       prev = l1 ++ [:: p] ++ l2 /\
       p \notin l1 /\
       Z.of_nat (size (undup_fst prev)) -
-      Z.of_nat (size (undup_fst l1)).+1 > threshold).
+      Z.of_nat (size (undup_fst l1)).+1 > threshold) /\
+  (*All received packets are in blks2*)
+  (forall (p: fpacket), p \in prev -> exists (b: block),
+    (b \in blks2) && packet_in_block p b) /\
+  (*All blocks are subblocks of [get_blocks] of the received stream*)
+  (forall b, b \in blks2 -> exists b', b' \in (get_blocks prev) /\
+    subblock b b').
 (*This is very very similar to the decoder invariant - does it
   follow? Should we change? see*)
 
@@ -591,14 +589,630 @@ Definition to_nto_invar (blks1 blks2 : list block)
       result of each still satisfies this invariant
     maybe combine these proofs
     then lift to multiple and/or all steps*)
+(*Search find.*)
+(*Let's think about this: maybe we should rewrite [upd_dec_state_gen]
+  as something like: 
+  if (has blks (fun b => blockId b = fd_blockId p)) then
+  let b := nth (find (fun b => ...)) blks in
+  insert (add_packet_to_block p b) (remove b blks) else
+  insert (new_packet_with_block p time) blks
+
+  then we can reason about \in more directly without induction
+  
+  let n := find (blockId =fd_blockId p) blks in
+    if
+    *)
+
+(*Idea: lemma: if block with id = fd_blockId p is
+  equal, then update_dec_state .2 is equal*)
+(*Lemma *)
+
+Lemma len1: forall (n: nat),
+  (n <= 1)%N = (n == 0)%N || (n == 1)%N.
+Proof.
+  move=> n. case: n=>//= n'.
+  by rewrite ltn1.
+Qed.
+ (*If there is only at most 1 element satisfying a predicate in a list,
+  then any two elements in the last satisfying the predicate must be
+  equal*)
+Lemma nth_uniq_eq: forall {A: eqType} (s: seq A) (p: pred A) (x y: A),
+  (count p s <= 1)%N ->
+  p x ->
+  p y ->
+  x \in s ->
+  y \in s ->
+  x = y.
+Proof.
+  (*TODO: in ListPoly, move size1P to CommonSSR*)
+  move=> A s p x y. rewrite -size_filter len1 => /orP[/eqP Hnil | 
+    /ListPoly.size1P [z Hs]] Hpx Hpy Hinx Hiny.
+  - apply size0nil in Hnil.
+    have: x \in [seq x <- s | p x] by rewrite mem_filter Hpx.
+    by rewrite Hnil.
+  - have: x \in [seq x <- s | p x] by rewrite mem_filter Hpx.
+    have: y \in [seq x <- s | p x] by rewrite mem_filter Hpy.
+    rewrite !Hs !in_cons !orbF => /eqP Hyz /eqP Hxz.
+    by rewrite Hyz Hxz.
+Qed.
+
+Lemma find_uniq_eq: forall {A: eqType} (s1 s2: seq A) (p: pred A) (d: A),
+  (count p s1 <= 1)%N ->
+  (count p s2 <= 1)%N ->
+  has p s1 ->
+  has p s2 ->
+  (forall x, x \in s1 -> x \in s2) ->
+  nth d s1 (find p s1) = nth d s2 (find p s2).
+Proof.
+  move=> A s1 s2 p def Hc1 Hc2 Hhas1 Hhas2 Hsub.
+  case: (findP p s1). by rewrite Hhas1.
+  move=> i1 Hi1 Hnth1 Hbef1.
+  case: (findP p s2). by rewrite Hhas2.
+  move=> i2 Hi2 Hnth2 Hbef2.
+  have Hin1: nth def s1 i1 \in s1 by apply mem_nth.
+  have Hin2: nth def s1 i1 \in s2 by apply Hsub.
+  have Hin2': nth def s2 i2 \in s2 by apply mem_nth.
+  by apply (nth_uniq_eq Hc2).
+Qed.
+
+(*Finally, prove that sorted by blk_order implies count <= 1*)
+Lemma blk_count: forall (blks: list block) (n: nat),
+  sorted blk_order blks ->
+  (count (fun b => blk_id b == n) blks <= 1)%N.
+Proof.
+  move=> blks n.
+  elim: blks => [// | bhd btl /= IH].
+  rewrite path_sortedE; last by apply blk_order_trans.
+  move=> /andP[/allP Hall Hsort].
+  case: (blk_id bhd == n) /eqP => Hhd/=; last by apply IH.
+  have->//:count (fun b : block => blk_id b == n) btl = 0%N.
+  apply /eqP. apply negbFE. rewrite -lt0n -has_count.
+  apply negbTE. apply /hasP => [[b Hinb] /eqP Hidb].
+  have: (blk_id bhd < blk_id b)%N by apply Hall.
+  by rewrite Hidb Hhd ltnn.
+Qed.
+
+Lemma blk_order_irrefl: irreflexive blk_order.
+Proof.
+  move=> b. by rewrite /blk_order ltnn.
+Qed.
+
+Lemma blk_order_sort_uniq: forall blks,
+  sorted blk_order blks ->
+  uniq blks.
+Proof.
+  move=> blks. apply sorted_uniq.
+  apply blk_order_trans.
+  apply blk_order_irrefl.
+Qed.
+
+Lemma orb_notfirst: forall (b1 b2: bool),
+  b1 || b2 = b1 || (~~ b1 && b2).
+Proof.
+  move=> b1 b2. by case: b1.
+Qed. 
 
 
 (*maybe do as 1 step*)
-Lemma decoder_timeout_notimeout_blocks: 
-  forall blks1 blks2 prev packets sent1 sent2 time1 time2,
-  (forall (p: fpacket) (b: block), p \in packets -> 
-    b \in blks1 -> fd_blockId p = blk_id b -> 
-    b \in blks2) ->
+Lemma decoder_timeout_notimeout_one: 
+  forall blks1 blks2 prev p time,
+  to_nto_invar blks1 blks2 prev ->
+  wf_packet_stream (prev ++ [:: p]) ->
+  reorder_dup_cond (prev ++ [:: p]) ->
+  decoder_timeout_invar blks1 prev time ->
+  sorted blk_order blks2 ->
+  (*The outputs are equal*)
+  (decoder_one_step blks1 p time).1.2 =
+  (decoder_one_step_gen upd_time triv_timeout blks2 p time).1.2 /\
+  (*The blocks mantain the invariant*)
+  to_nto_invar (decoder_one_step blks1 p time).1.1
+    (decoder_one_step_gen upd_time triv_timeout blks2 p time).1.1 
+    (prev ++ [:: p]) /\
+  (*The updated times are equal*)
+  (decoder_one_step blks1 p time).2 =
+  (decoder_one_step_gen upd_time triv_timeout blks2 p time).2.
+Proof.
+  move=> blks1 blks2 prev p time Hinvar Hwf Hcond Hdecinv Hsort2.
+  have Hwfcons: wf_packet_stream (p :: prev) by
+    apply (wf_perm Hwf); rewrite cats1 perm_rcons perm_refl.
+  have Hwf': wf_packet_stream prev by
+    apply (wf_packet_stream_tl Hwfcons).
+  (*Some results that are useful, since there are several impossible
+    cases from timeouts we use multiple times*)
+  (*1. The block in blks2 with p's id is in blks1*)
+  have Hbpin21: forall b,
+    b \in blks2 -> blk_id b = fd_blockId p ->
+    b \in blks1. {
+    move=> b Hinb Hid. 
+    case Hinb1: (b \in blks1)=>//.
+    have Hbnot: b \notin blks1 by rewrite Hinb1.
+    case: Hinvar => [Hb12 [Hnotb12 Hsubs]].
+    move: Hnotb12 => /(_ b Hinb Hbnot) 
+      [p' [l1 [l2 [Hidp' [Hprev [Hnotin Htimeout]]]]]].
+    exfalso. apply (@same_block_close prev p p' l1 l2)=>//; first
+      by rewrite Hidp' Hid.
+    have->: (l1 ++ [:: p'] ++ l2 ++ [:: p]) = prev ++ [:: p]
+      by rewrite Hprev !catA.
+    rewrite !undup_fst_rcons (negbTE Hnotin).
+    case Hinp: (p \in prev); rewrite !size_cat !addn1; lia.
+  }
+  (*2: The block in blks2 containing p (if one exists), is in blks1*)
+  have Hbpin21': forall b,
+    b \in blks2 ->
+    packet_in_block p b ->
+    b \in blks1. {
+    move=> b Hinb Hinp.
+    apply Hbpin21 =>//. symmetry. by apply (decoder_invar_allid Hwf' 
+      (proj2 (proj2 (proj2 Hinvar)))).   
+    }
+  (*Sorted lemmas*)
+  have Hsort1': sorted blk_order 
+    [seq x <- blks1 | not_timed_out (upd_time time p blks1) x] by
+    (apply sorted_filter; [apply blk_order_trans | apply Hdecinv]).
+  have Hsort2': sorted blk_order 
+    [seq x <- blks2 | triv_timeout (upd_time time p blks2) x] by
+    (apply sorted_filter=>//; apply blk_order_trans).
+  (*Can we provethis?*)
+  have Hupdtime: upd_time time p blks1 = 
+    if p \in prev then time else time + 1. {
+      rewrite upd_time_spec.
+      - case: (existsb [eta packet_in_block p] blks1) /existsbP => 
+        [[b /andP[Hinb1 Hidb1]] | Hnotex1].
+        + have->//=: p \in prev. eapply (decoder_invar_inprev Hwf').
+          apply Hdecinv. apply Hinb1. by [].
+        + (*We can prove this*)
+          case Hin: (p \in prev)=>//.
+          move: Hinvar => [_ [_ [/(_ p Hin) [b' /andP[Hinb' Hinp]] _]]].
+          exfalso. apply Hnotex1. exists b'. rewrite Hinp andbT.
+          by apply Hbpin21'.
+      - apply Hdecinv.
+      - apply (decoder_invar_allid Hwf'). apply Hdecinv.
+  }
+  (*We need the time invariant for the output result*)
+  have Htimes: upd_time time p blks1 = upd_time time p blks2. {
+    rewrite Hupdtime upd_time_spec.
+    - case: (existsb [eta packet_in_block p] blks2) /existsbP => 
+      [[b /andP[Hinb2 Hidb2]] | Hnotex1].
+      + have->//: p \in prev. 
+        eapply (decoder_invar_inprev Hwf') with(b:=b)=>//.
+        2: apply Hinb2. apply Hinvar.
+      + case Hin: (p \in prev)=>//.
+        move: Hinvar => [_ [_ [/(_ p Hin) [b' /andP[Hinb' Hinp] _]]]].
+        exfalso. apply Hnotex1. exists b'. by rewrite Hinb'.
+    - apply Hsort2.
+    - apply (decoder_invar_allid Hwf'). apply Hinvar.
+  } 
+  rewrite /=.
+  rewrite -and_assoc. split=>//.
+  (*Handle the 2 easier ones first*)
+  rewrite /to_nto_invar -!and_assoc. split; last first.
+    (*easy and same as above: maybe separate lemma*)
+    move=> b Hinb.
+    (*need permutation*)
+    have [b' [Hinb' Hsub]]: exists (b': block), 
+      b' \in get_blocks (p :: prev) /\ subblock b b' :=
+      (decoder_one_step_gen_subblocks Hwfcons 
+        (proj2 (proj2 (proj2 Hinvar))) Hinb).
+    have Hperm: perm_eq (get_blocks (p :: prev)) 
+      (get_blocks (prev ++ [:: p])). {
+        apply get_blocks_perm=>//. 
+        by rewrite cats1 -perm_rcons perm_refl.
+      }
+    exists b'.
+    by rewrite -(perm_mem Hperm).
+  split; last first. {
+    (*TODO: maybe dont do this first, not as easy as I thought
+      do we need this for sure?*)
+    move=> p'.
+    rewrite mem_cat => /orP[Hprev | ]; last first.
+    - rewrite in_cons orbF => /eqP Hp; subst.
+      apply (packet_in_one_step _ _ _ Hwf).
+      + by rewrite mem_cat in_cons eq_refl orbT.
+      + (*NOTE: copied this - bad*) 
+      move=> b1 p1 Hinp1 Hinb1 Hids.
+      case: Hinvar => [_ [_ [_ /( _ _ Hinb1) [b2 [Hinb2 Hsub]]]]].
+      (*Not quite enough, need a block from [get_blocks (prev ++ [:: p])]*)
+      have Hsubstream: (forall (x: fpacket), x \in prev -> 
+        x \in prev ++ [:: p]) by move=> x; rewrite mem_cat=>->.
+      have [b3 [Hinb3 Hsub2]]:=(get_blocks_sublist Hwf Hsubstream Hinb2).
+      have Hsub3 :=(subblock_trans Hsub Hsub2).
+      have Hideq: blk_id b1 = blk_id b3 by apply Hsub3.
+      rewrite Hideq in Hids. rewrite {Hideq}.
+      have[-> ->]:blk_k b1 = blk_k b3 /\ blk_h b1 = blk_h b3 by apply Hsub3.
+      apply (get_blocks_kh Hwf)=>//. by rewrite mem_cat mem_head orbT.
+      + (*also copied BAD - need proof that subblock implies
+          these as separate lemma*)
+        move=> b' Hinb'.
+        case: Hinvar => [_ [_ [_ /( _ _ Hinb') 
+          [b'' [Hinb'' [Hids [Hdat [Hpars [Hk Hh]]]]]]]]].
+        rewrite Hk Hh (proj1 Hdat) (proj1 Hpars).
+        by apply (get_blocks_Zlength Hwf').
+    - rewrite update_dec_state_gen_eq //.
+      rewrite /=/triv_timeout/=.
+      rewrite filter_predT.
+      case Hhas: (has (fun b0 : block => blk_id b0 == fd_blockId p) blks2).
+      + have:=Hhas => /hasP [b Hinb /eqP Hidb].
+        case: (fd_blockId p' == fd_blockId p) /eqP => Hids/=.
+        * exists (add_packet_to_block_black p
+        (nth block_inhab blks2
+           (find (fun b1 : block => blk_id b1 == fd_blockId p) blks2))).1.
+          rewrite mem_insert eq_refl/=. 
+          (*ugh: continue with this: we know there is some block
+            that contains p' by IH, it is the same as nth find
+            because of uniquenss. Only way p' could not
+            be in is if blockIndex equals, but then p' is p, so good*)
+          admit.
+        * (*From IH, know it cannot equal add_black bc id different
+            and will be in rem before not same ID*)
+          admit.
+      + rewrite /=. (*since false, use IH, cannot be
+        in same as p or else there would be a block in blks2
+        with id, contradict HHas*)
+        admit.
+  }        
+        
+  rewrite !and_assoc !update_dec_state_gen_eq //.
+  (*See if there is a block with p's ID inside blks2*)
+  case Hhas2: (has (fun b : block => blk_id b == fd_blockId p)
+    [seq x <- blks2 | triv_timeout (upd_time time p blks2) x]).
+  - have:=Hhas2 => /hasP [b]. 
+    rewrite mem_filter => /andP[_ Hinb2] /eqP Hidb. 
+    (*We know that this block is also in blks1*)
+    have Hinb1: b \in blks1 by apply Hbpin21.
+    (*See if it has timed out or not*)
+    case Hto: (not_timed_out (upd_time time p blks1) b).
+    + (*If it timed out, "has" is true*)
+      have Hhas1: has (fun b0 : block => blk_id b0 == fd_blockId p)
+      [seq x <- blks1 | not_timed_out (upd_time time p blks1) x]. {
+        apply /hasP. exists b. by rewrite mem_filter Hto. 
+        by rewrite Hidb.
+      }
+      rewrite Hhas1.
+      (*This result is needed in multiple places:*)
+      have Hntheq: 
+      nth block_inhab [seq x <- blks1 | not_timed_out (upd_time time p blks1) x]
+      (find (fun b0 : block => blk_id b0 == fd_blockId p)
+         [seq x <- blks1 | not_timed_out (upd_time time p blks1) x]) =
+      nth block_inhab [seq x <- blks2 | triv_timeout (upd_time time p blks2) x]
+      (find (fun b0 : block => blk_id b0 == fd_blockId p)
+         [seq x <- blks2 | triv_timeout (upd_time time p blks2) x]). {
+        apply find_uniq_eq=>//; last by
+        move=> x; rewrite !mem_filter/= =>/andP[_ Hinx];
+        apply Hinvar.
+        all: apply blk_count; apply sorted_filter=>//; try apply
+          blk_order_trans.
+        apply Hdecinv.
+      }
+      (*Now we prove each result in turn*)
+      split_all=>//.
+      * by rewrite/= Hntheq.
+      * move =>/= b'.
+        rewrite !mem_insert Hntheq => /orP[/eqP Hb | Hinrest]; first
+        by rewrite Hb eq_refl.
+        apply /orP. right. move: Hinrest. 
+        rewrite !mem_rem_uniq.
+        -- rewrite /in_mem/= => /andP[Hbnot].
+          rewrite Hbnot !mem_filter/= => /andP[_ Hinb']. by apply Hinvar.
+        -- apply (blk_order_sort_uniq Hsort2').
+        -- apply (blk_order_sort_uniq Hsort1'). 
+      * move=> b'.
+        rewrite !mem_insert !Hntheq => 
+          /orP[/eqP Hb | Hinrest2]; first by
+          rewrite Hb eq_refl.
+        rewrite negb_orb => /andP[Hneq Hnotinrest].
+        move: Hnotinrest Hinrest2. rewrite !mem_rem_uniq;
+          [|apply (blk_order_sort_uniq Hsort2')|
+            apply (blk_order_sort_uniq Hsort1')].
+        setoid_rewrite <- addn1. (*to stop simpl*)
+        rewrite /in_mem/=. rewrite negb_and => Htemp /andP[Hneq' Hinb2'].
+        move: Hinb2'. rewrite mem_filter/==> Hinb2'.
+        move: Htemp. rewrite Hneq'/= mem_filter.
+        rewrite negb_and => /orP[Htimeout | Hnotin]; last first.
+        -- (*from IH*)
+          move: Hinvar => [_ [/( _ _ Hinb2' Hnotin) 
+            [p' [l1 [l2 [Hids [Hprev [Hnotinp' Hthresh]]]]]] _]].
+          exists p'. exists l1. exists (l2 ++ [:: p]).
+          split_all=>//. by rewrite Hprev -!catA. rewrite addn1.
+          rewrite undup_fst_rcons.
+          case Hin: (p \in prev); first by apply Hthresh.
+          move: Hthresh.
+          rewrite size_cat addn1 !Nat2Z.inj_succ. simpl in *; lia.
+        -- (*Now we have the timeout case: TODO: separate lemma*)
+          (*TODO: *)
+          move: Htimeout. rewrite /not_timed_out Z.leb_antisym => Htimeout.
+          rewrite negbK in Htimeout.
+          move: Htimeout => /Z.ltb_spec0 Htimeout.
+          (*OK, we still need to know that blocks in blks2
+            have a packet which has the time of arrival*)
+            (*TODO: start with this tomorrow*)
+          
+
+          Print decoder_timeout_invar.
+          (*Idea: put new invariant that all blocks in blks
+            are not timed out- can show preserved very easily
+            then: we know that b' was not timed out,
+            so it must be the case that p was a new packet not
+            in an existing block and the time *)
+
+
+
+          eapply Zgt_trans. 2: apply Hthresh.
+          move: Ht
+          have: 
+          Search (?x - ?y <= ?z + ?w)%Z.
+          
+          lia.
+          move: Hthresh.
+        
+          
+          rewrite /=. lia.
+
+        have Hinb1': b' \in blks1.
+        
+        Hinb1.
+
+        Search (negb ())
+        
+      
+      rewrite /=.
+        
+        apply Hin. by [].
+
+  
+  - (*This*)
+  split_all=>//.
+  - rewrite /= !update_dec_state_gen_eq //=. 
+    (*See if there is a block with p inside blks1*)
+    (*TODO: case before split?*)
+    case : (existsb (fun b => blk_id b == fd_blockId p) blks1) /existsbP 
+      =>// [[b /andP[Hinb /eqP Hbid]] | Hnotex].
+    + (*This block is definitely in blks2*)
+      have Hinb2: b \in blks2 by apply Hinvar.
+      have Hhas2: (has (fun b0 : block => blk_id b0 == fd_blockId p)
+        [seq x <- blks2 | triv_timeout (upd_time time p blks2) x]).
+        apply /hasP. exists b. by rewrite mem_filter/=. by rewrite Hbid.
+      rewrite Hhas2.
+      (*Now we see if this block (or any block) is in blks1 after timeouts*)
+      case Hto: (not_timed_out (upd_time time p blks1) b).
+      * (*If it was, then we have the "has" predicate*)
+        have Hhas1: (has (fun b0 : block => blk_id b0 == fd_blockId p)
+        [seq x <- blks1 | not_timed_out (upd_time time p blks1) x]).
+          apply /hasP. exists b. by rewrite mem_filter Hto.
+          by rewrite Hbid.
+        rewrite Hhas1/=.
+        (*Now, we can show that the two blocks are equal
+        TODO: make separate lemma or maybe change case and split*)
+        f_equal. f_equal.
+        apply find_uniq_eq=>//; last by
+          move=> x; rewrite !mem_filter/= =>/andP[_ Hinx];
+          apply Hinvar.
+        all: apply blk_count; apply sorted_filter=>//; try apply
+          blk_order_trans.
+        apply Hdecinv.
+      * (*If not, then we have a timed out block, so we can
+        use the [decoder_timeout_invar] to get a packet that
+        arrived too long ago*)
+        exfalso. move: Hto. rewrite upd_time_spec; 
+          [| apply Hdecinv| apply (decoder_invar_allid Hwf'); apply Hdecinv].
+        rewrite /not_timed_out Z.leb_antisym => Hto. 
+        apply negbFE in Hto.
+        move: Hto => /Z.ltb_spec0 Hto.
+        case: Hdecinv => [Htime [Hstart [Htimed [Hsort Hsubs]]]].
+        move: Hto.
+        rewrite Htime. move: Hstart => /( _ b Hinb) 
+          [p' [l1 [l2 [Hidp' [Hprev [Hnotin Hblackt]]]]]].
+        rewrite -Hblackt => Hto.
+        apply (@same_block_close prev p p' l1 l2) =>//.
+          by rewrite Hidp' Hbid.
+        have->:(l1 ++ [:: p'] ++ l2 ++ [:: p]) = prev ++ [:: p]
+          by rewrite Hprev !catA.
+        rewrite !undup_fst_rcons (negbTE Hnotin) size_cat addn1.
+        move: Hto.
+        case : (existsb [eta packet_in_block p] blks1) /existsbP => 
+          [[b' /andP[Hinb' Hidb']] | ].
+        {
+          have->//: p \in prev; try lia. by apply (decoder_invar_inprev Hwf' Hsubs Hinb'). 
+        }
+        move => Hnotex.
+        case Hinp: (p \in prev); last by rewrite size_cat addn1; lia.
+        (*In this case, we use the 3rd decoder invariant to get
+          our contradiction - TODO reduce duplication*)
+        exfalso. clear -Htimed Hinp Hnotex Hcond.
+        move: Htimed => /(_ _ Hinp Hnotex) 
+          [p' [l1 [l2 [Hids [Hprev [Hnotin Htimeout]]]]]].
+        apply (@same_block_close prev p p' l1 l2)=>//.
+        have->:(l1 ++ [:: p'] ++ l2 ++ [:: p]) = prev ++ [:: p]
+          by rewrite Hprev !catA.
+        by rewrite !undup_fst_rcons (negbTE Hnotin) Hinp size_cat addn1.
+    + (*Now there is nothing inside blks1. *)
+      have Hhas1: has (fun b : block => blk_id b == fd_blockId p)
+      [seq x <- blks1 | not_timed_out (upd_time time p blks1) x] = false. {
+        apply negbTE. apply /hasP. move=> [x Hx Hxid]. apply Hnotex.
+        exists x. move: Hx. rewrite mem_filter => /andP[_ Hinx].
+        by rewrite Hinx Hxid.
+      }
+      rewrite Hhas1.
+      (*Now we determine if there is a block with this idx in
+        blks2.*)
+      case: (existsb (fun b => blk_id b == fd_blockId p) blks2) /existsbP 
+      =>// [[b /andP[Hinb /eqP Hbid]] | Hnotex2]; last first.
+      * (*If not, then easy to show that these are equal*)
+        have Hhas2: ( has (fun b : block => blk_id b == fd_blockId p)
+        [seq x <- blks2 | triv_timeout (upd_time time p blks2) x] = false). {
+          apply negbTE. apply /hasP. move=> [x Hx Hxid]. apply Hnotex2.
+          exists x. move: Hx. rewrite mem_filter => /andP[_ Hinx].
+          by rewrite Hinx Hxid.
+        }
+        rewrite Hhas2/=.
+        (*Need to know time invariant here*)
+        by rewrite Htimes.
+      * (*If there is, then we get a contradiction since a packet
+          appeared too long ago*)
+        exfalso. apply Hnotex. exists b. rewrite Hbid eq_refl andbT.
+        by apply Hbpin21.
+  - (*Now we prove that the invariant is preserved*)  
+    rewrite /to_nto_invar; split_all; last first.
+    + 
+    + move=> b.
+      rewrite !update_dec_state_gen_eq //.
+      (*Once again, we proceed by cases (TODO: should we do
+        cases like this? i think so - should refactor)*)
+      case Hhas2: 
+
+
+
+          NOTE: Here is by blockID
+          
+          so idea:
+          1. for any block in blks1, blk_id b == fd_blockId p =
+            (p \in prev ==> packet_in_block p b)
+
+          2. have block with p's id in blks2 ->
+              no block with p's id in blks1 ->
+              contradiction
+
+          3. have block with p's id in blks2 <-> block with p's id in blks1
+
+          4. therefore, have block that p is in blks2 ->
+
+          
+          *)
+
+
+
+        lia.
+
+
+        have Hcon: black_time b + threshold < time + 1 -> False; last first.
+           apply Hcon. move: Hto. case: (existsb [eta packet_in_block p] blks1); lia.
+        case: Hdecinv => [Htime [Hstart [Htimed [Hsort Hsubs]]]].
+        rewrite Htime. move: Hstart => /( _ b Hinb) 
+          [p' [l1 [l2 [Hidp' [Hprev [Hnotin Hblackt]]]]]].
+        rewrite -Hblackt => Hto'.
+        apply (@same_block_close prev p p' l1 l2) =>//.
+        by rewrite -Hbid Hidp'.
+        have->:(l1 ++ [:: p'] ++ l2 ++ [:: p]) = prev ++ [:: p]
+          by rewrite Hprev !catA.
+        rewrite !undup_fst_rcons (negbTE Hnotin).
+        (*lia is being annoying*)
+        have to'': Z.of_nat (size (undup_fst prev)) - 
+        Z.of_nat (size (undup_fst l1)) > threshold by lia.
+        case Hpin: (p \in prev); rewrite !size_cat/=.
+        {
+          rewrite Nat2Z.inj_add. lia.
+          Search (Z.of_nat (?x + ?y)%coq_nat).
+          eapply Zgt_trans. 2: apply to''.  lia.
+          Search Z.gt "trans".
+          eapply Z.gt_trans.
+        }
+        lia.
+        existsb [eta packet_in_block p] blks1
+
+        
+        
+          2: apply Hdecinv.
+        
+      + (*If not, then see if we have such a block in blks2*)
+        case Hhas2: (has (fun b : block => blk_id b == fd_blockId p)
+        [seq x <- blks2 | triv_timeout (upd_time time p blks2) x]).
+        * (*Here, we use the invariant to get a contradiction*)
+          move: Hhas2 => /hasP [b]; rewrite mem_filter => /andP[_ Hinb] /eqP Hbid.
+          (*packets too far apart - TODO: put previous lemma and 
+          generalize (or maybe just that one)*)
+          exfalso.
+          have Hnotin1: b \notin blks1. 
+          case: Hinvar => [_ /(_ b Hinb)].
+          apply (@same_block_close )
+
+    --  
+
+
+    (*case : (existsb (fun b => blk_id b == fd_blockId p) blks1) /existsbP 
+    =>// [[b /andP[Hinb /eqP Hbid]] | Hnotex].*)
+    + (*In this case, there is one inside blks2. Thus, these blocks
+      must be the same (TODO: make this a separate
+      lemma and use it later - we prove MORE than just about packet
+      output, prove that blocks are the same)*) 
+      have Hinb2: b \in blks2 by apply Hinvar.
+      rewrite !update_dec_state_gen_eq.
+      * case Hhas1: (has (fun b0 : block => blk_id b0 == fd_blockId p)
+        [seq x <- blks1 | not_timed_out (upd_time time p blks1) x]). 
+      -- have:= Hhas1 => /hasP [b'] Hinb' /eqP Hidb'. 
+        move: Hinb'. rewrite mem_filter => /andP[Htob' Hinb']/=.
+        have Hhas2: has (fun b0 : block => blk_id b0 == fd_blockId p)
+        [seq x <- blks2 | triv_timeout (upd_time time p blks2) x]. {
+          apply /hasP. exists b'. rewrite mem_filter/=.
+          by apply Hinvar. by rewrite Hidb'.
+        }
+        rewrite Hhas2/=. f_equal. f_equal.
+        apply find_uniq_eq=>//; last by
+          move=> x; rewrite !mem_filter/= =>/andP[_ Hinx];
+          apply Hinvar.
+        all: apply blk_count; apply sorted_filter=>//; try apply
+          blk_order_trans.
+        apply Hdecinv.
+      --  
+          
+        
+        
+        try (apply blk_count; apply sorted_filter=>//).
+
+        case: (findP (fun b0 : block => blk_id b0 == fd_blockId p)
+        [seq x <- blks1 | not_timed_out (upd_time time p blks1) x]).
+        by rewrite Hhas1. move => i1 Hi1 Hnth1 Hbefore1/=.
+        case: (findP (fun b0 : block => blk_id b0 == fd_blockId p)
+        [seq x <- blks2 | triv_timeout (upd_time time p blks2) x]).
+        by rewrite Hhas2. move=> i2 Hi2 Hnth2 Hbefore2/=.
+        (*Need to know that these two blocks are equal - TODO separate
+          lemma for some of this?*)
+        f_equal. f_equal. 
+
+        rewrite /=.
+        
+      
+      
+      rewrite
+
+
+      (*TODO: lemma above*) admit.
+    + (*maybe - lemma saying if none, then equal to insert (maybe)*)
+      (*Then we see if such a block is in blks2*)
+      case : (existsb (fun b => blk_id b == fd_blockId p) blks2) /existsbP 
+      =>// [[b /andP[Hinb /eqP Hbid]] | Hnotex2].
+      * move: Hinvar => [_ /(_ b Hinb)].
+        have->: b \notin blks1. case Hinb1: (b \in blks1) =>//.
+        exfalso. apply Hnotex. exists b. by rewrite Hinb1 Hbid eq_refl.
+        move=>/(_ isT) [p' [l1 [l2 [Hidp' [Hprev [Hnotin Htimeout]]]]]].
+        (*Here, we get a contradiction because packets too far apart*)
+        (*TODO: put previous result in separate lemma*)
+        admit.
+      * (*Here, we need a lemma that says about the insertion to
+        prove that they are equal: all we really need for this part is:
+        if no block, then packets outputted are those from (create_block_black))*)
+        admit.
+  - rewrite /to_nto_invar. split.
+    + (*Yeah, we will need some sort of lemma like above, let's try to
+      prove it*)
+
+  
+  
+  rewrite /=.
+  
+  move: blks1 Hinvar.
+  rewrite /decoder_one_step/=/triv_timeout. 
+  elim: blks2 => [//= [//= | bhd1 btl1] | bhd2 btl2 ].
+  - move=> _ Hinvar. split_all=>//.
+    rewrite /to_nto_invar/=. split=>//.
+    move=> b. by rewrite !in_cons orbF =>->.
+  - move=> Hinvar. exfalso.
+    move: Hinvar. rewrite /to_nto_invar => [[Hcon _]].
+    by move: Hcon => /(_ bhd1 (mem_head _ _)).
+  - move => Hinvar [//= ]. 
+    
+    
+    
+    => Hinv1. by []. 
+
   decoder_multiple_steps prev packets 
 
 
